Port comments to coq code

semtyping.v
@@ -3,10 +3,24 @@ From WR Require Import syntax join imports.
 Definition ProdSpace (PA : tm -> Prop) (PF : tm -> (tm -> Prop) -> Prop) (b : tm) :=
   forall a PB, PA a -> PF a PB -> PB (tApp b a).
 
+(* Logical Relation:
+
+  InterpUnivN i A P  holds when
+   - A is a Set i
+   - P is a predicate on terms that act like type A
+
+  We define this in two parts: one that generalizes over
+  smaller interpretations and then tie the knot
+  with the real definition below.
+
+ *)
+
+Notation predeq P Q := (forall x, P x <-> Q x).
+
 Inductive InterpExt n (I : nat -> tm -> Prop) : tm -> (tm -> Prop) -> Prop :=
 | InterpExt_Void : InterpExt n I tVoid (const False)
 | InterpExt_Bool : InterpExt n I tBool (fun a => exists v, Pars a v /\ is_bool_val v)
-| InterpExt_Fun A B PA (PF : tm -> (tm -> Prop) -> Prop) :
+| InterpExt_Fun A B PA PF :
   InterpExt n I A PA ->
   (forall a, PA a -> exists PB, PF a PB) ->
   (forall a PB, PF a PB -> InterpExt n I (subst_tm (a..) B) PB) ->
@@ -20,14 +34,6 @@ Inductive InterpExt n (I : nat -> tm -> Prop) : tm -> (tm -> Prop) -> Prop :=
   Par A A0 ->
   InterpExt n I A0 PA ->
   InterpExt n I A PA.
-
-Lemma InterpExt_Fun_nopf n I A B PA  :
-  InterpExt n I A PA ->
-  (forall a, PA a -> exists PB, InterpExt n I (subst_tm (a..) B) PB) ->
-  InterpExt n I (tPi A B) (ProdSpace PA (fun a => InterpExt n I (subst_tm (a..) B))).
-Proof.
-  move => h0 h1. apply InterpExt_Fun =>//.
-Qed.
 
 Lemma InterpExt_Eq' n I PA a b A :
   PA = (fun p => Pars p tRefl /\ Coherent a b) ->
@@ -47,6 +53,62 @@ Equations InterpUnivN (n : nat) : tm -> (tm -> Prop) -> Prop by wf n lt :=
                                   | right _ => False
                                   end).
 
+(* ---------------------------------------------------- *)
+
+(* The definition of InterpUnivN is more complicated than
+   it needs to be. We show that that we can
+   simplify the unfolding above to just mention InterpUnivN
+   without doing the case analysis.
+*)
+Lemma InterpExt_lt_redundant n I A PA
+  (h : InterpExt n I A PA) :
+      InterpExt n (fun m A =>
+                     match Compare_dec.lt_dec m n with
+                     | left h => I m A
+                     | right _ => False
+                     end) A PA.
+Proof.
+  elim : A PA / h.
+  - hauto l:on.
+  - hauto l:on.
+  - hauto l:on ctrs:InterpExt.
+  - move => m h.
+    apply InterpExt_Univ' => //.
+    case : Compare_dec.lt_dec => //.
+  - hauto l:on.
+  - hauto lq:on ctrs:InterpExt.
+Qed.
+
+Lemma InterpExt_lt_redundant2 n I A PA
+  (h : InterpExt n (fun m A =>
+                      match Compare_dec.lt_dec m n with
+                     | left h => I m A
+                     | right _ => False
+                     end) A PA) :
+  InterpExt n I A PA.
+Proof.
+  elim : A PA / h.
+  - hauto l:on.
+  - hauto l:on.
+  - hauto l:on ctrs:InterpExt.
+  - move => m ?.
+    apply InterpExt_Univ' => //.
+    case : Compare_dec.lt_dec => //.
+  - hauto l:on.
+  - hauto lq:on ctrs:InterpExt.
+Qed.
+
+Lemma InterpUnivN_nolt n :
+  InterpUnivN n = InterpExt n (fun m A => exists PA, InterpUnivN m A PA).
+Proof.
+  simp InterpUnivN.
+  fext => A P.
+  apply propositional_extensionality.
+  hauto l:on use:InterpExt_lt_redundant, InterpExt_lt_redundant2.
+Qed.
+
+#[export]Hint Rewrite InterpUnivN_nolt : InterpUniv.
+
 Lemma InterpExt_Fun_inv n I A B P  (h : InterpExt n I (tPi A B) P) :
   exists (PA : tm -> Prop) (PF : tm -> (tm -> Prop) -> Prop),
     InterpExt n I A PA /\
@@ -61,6 +123,53 @@ Proof.
   - move => *; subst.
     hauto lq:on inv:Par ctrs:InterpExt use:par_subst.
 Qed.
+
+
+(* For all of the proofs about InterpUnivN below, we need to
+   do them in two steps. Once for InterpExt, and then tie the
+   knot for the full definition. *)
+
+(* -----  I-PiAlt is admissible (free of PF, the relation R on paper)  ---- *)
+
+Lemma InterpExt_Fun_nopf n I A B PA  :
+  InterpExt n I A PA ->
+  (forall a, PA a -> exists PB, InterpExt n I (subst_tm (a..) B) PB) ->
+  InterpExt n I (tPi A B) (ProdSpace PA (fun a => InterpExt n I (subst_tm (a..) B))).
+Proof.
+  move => h0 h1. apply InterpExt_Fun =>//.
+Qed.
+
+Lemma InterpUnivN_Fun_nopf n A B PA :
+  InterpUnivN n A PA ->
+  (forall a, PA a -> exists PB, InterpUnivN n (subst_tm (a..) B) PB) ->
+  InterpUnivN n (tPi A B) (ProdSpace PA (fun a => InterpUnivN n (subst_tm (a..) B))).
+Proof.
+  hauto l:on use:InterpExt_Fun_nopf rew:db:InterpUniv.
+Qed.
+
+(* --------------- relation is cumulative ----------------- *)
+
+Lemma InterpExt_cumulative n m I A PA :
+  n < m ->
+  InterpExt n I A PA ->
+  InterpExt m I A PA.
+Proof.
+  move => h h0.
+  elim : A PA /h0;
+    hauto l:on ctrs:InterpExt use:PeanoNat.Nat.lt_trans.
+Qed.
+
+Lemma InterpUnivN_cumulative n A PA :
+  InterpUnivN n A PA -> forall m, n < m ->
+  InterpUnivN m A PA.
+Proof.
+  hauto l:on rew:db:InterpUniv use:InterpExt_cumulative.
+Qed.
+
+(* ------------------------------------------------------- *)
+
+(* The logical relation is closed under parallel reduction,
+   forwards and backwards. *)
 
 Lemma InterpExt_preservation n I A B P (h : InterpExt n I A P) :
   Par A B ->
@@ -115,12 +224,18 @@ Lemma InterpUnivN_back_preservation_star n A B P (h : InterpUnivN n B P) :
   InterpUnivN n A P.
 Proof. hauto l:on rew:db:InterpUnivN use:InterpExt_back_preservation_star. Qed.
 
+(* ---------------------------------------------------------- *)
+
 Lemma InterpUnivN_Coherent n A B P (h : InterpUnivN n B P) :
   Coherent A B ->
   InterpUnivN n A P.
 Proof.
   hauto l:on unfold:Coherent use:InterpUnivN_back_preservation_star, InterpUnivN_preservation_star.
 Qed.
+
+(* ---------------------------------------------------------- *)
+(* inversion lemmas for InterpExt. To invert the InterpExt
+   judgment, we have to be careful about the step case. *)
 
 Lemma InterpExt_Bool_inv n I P :
   InterpExt n I tBool P ->
@@ -171,6 +286,8 @@ Proof.
   hauto lq:on use:Par_Coherent, Coherent_symmetric, Coherent_transitive.
 Qed.
 
+(* ------------- relation is deterministic ---------------- *)
+
 Lemma InterpExt_deterministic n I A PA PB :
   InterpExt n I A PA ->
   InterpExt n I A PB ->
@@ -193,6 +310,39 @@ Proof.
   - hauto l:on use:InterpExt_preservation.
 Qed.
 
+Lemma InterpUnivN_deterministic n A PA PB :
+  InterpUnivN n A PA ->
+  InterpUnivN n A PB ->
+  PA = PB.
+Proof.
+  simp InterpUnivN. apply InterpExt_deterministic.
+Qed.
+
+(* slight generalization to work with any levels using cumulativity. *)
+
+Lemma InterpExt_deterministic' n m I A PA PB :
+  InterpExt n I A PA ->
+  InterpExt m I A PB ->
+  PA = PB.
+Proof.
+  move => h0 h1.
+  case : (Coq.Arith.Compare_dec.lt_eq_lt_dec m n); first case.
+  - hauto l:on use:InterpExt_cumulative, InterpExt_deterministic.
+  - move => *; subst.
+    sfirstorder use:InterpExt_deterministic.
+  - move => ?.
+    symmetry.
+    hauto l:on use:InterpExt_cumulative, InterpExt_deterministic.
+Qed.
+
+Lemma InterpUnivN_deterministic' n m  A PA PB :
+  InterpUnivN n A PA ->
+  InterpUnivN m A PB ->
+  PA = PB.
+Proof. hauto lq:on rew:off use:InterpExt_deterministic' rew:db:InterpUniv. Qed.
+
+(* ----- Improved inversion lemma for functions (Pi Inv Alt) ---------- *)
+
 Lemma InterpExt_Fun_inv_nopf n I A B P  (h : InterpExt n I (tPi A B) P) :
   exists (PA : tm -> Prop),
     InterpExt n I A PA /\
@@ -210,82 +360,6 @@ Proof.
     + sfirstorder.
 Qed.
 
-Lemma InterpUnivN_deterministic n A PA PB :
-  InterpUnivN n A PA ->
-  InterpUnivN n A PB ->
-  PA = PB.
-Proof.
-  simp InterpUnivN.
-  eauto using InterpExt_deterministic.
-Qed.
-
-Lemma InterpExt_cumulative n m I A PA :
-  n < m ->
-  InterpExt n I A PA ->
-  InterpExt m I A PA.
-Proof.
-  move => h h0.
-  elim : A PA /h0;
-    hauto l:on ctrs:InterpExt use:PeanoNat.Nat.lt_trans.
-Qed.
-
-Lemma InterpExt_lt_redundant n I A PA
-  (h : InterpExt n I A PA) :
-      InterpExt n (fun m A =>
-                     match Compare_dec.lt_dec m n with
-                     | left h => I m A
-                     | right _ => False
-                     end) A PA.
-Proof.
-  elim : A PA / h.
-  - hauto l:on.
-  - hauto l:on.
-  - hauto l:on ctrs:InterpExt.
-  - move => m h.
-    apply InterpExt_Univ' => //.
-    case : Compare_dec.lt_dec => //.
-  - hauto l:on.
-  - hauto lq:on ctrs:InterpExt.
-Qed.
-
-Lemma InterpExt_lt_redundant2 n I A PA
-  (h : InterpExt n (fun m A =>
-                      match Compare_dec.lt_dec m n with
-                     | left h => I m A
-                     | right _ => False
-                     end) A PA) :
-  InterpExt n I A PA.
-Proof.
-  elim : A PA / h.
-  - hauto l:on.
-  - hauto l:on.
-  - hauto l:on ctrs:InterpExt.
-  - move => m ?.
-    apply InterpExt_Univ' => //.
-    case : Compare_dec.lt_dec => //.
-  - hauto l:on.
-  - hauto lq:on ctrs:InterpExt.
-Qed.
-
-Lemma InterpUnivN_nolt n :
-  InterpUnivN n = InterpExt n (fun m A => exists PA, InterpUnivN m A PA).
-Proof.
-  simp InterpUnivN.
-  fext => A P.
-  apply propositional_extensionality.
-  hauto l:on use:InterpExt_lt_redundant, InterpExt_lt_redundant2.
-Qed.
-
-#[export]Hint Rewrite InterpUnivN_nolt : InterpUniv.
-
-Lemma InterpUnivN_Fun n A B PA :
-  InterpUnivN n A PA ->
-  (forall a, PA a -> exists PB, InterpUnivN n (subst_tm (a..) B) PB) ->
-  InterpUnivN n (tPi A B) (ProdSpace PA (fun a => InterpUnivN n (subst_tm (a..) B))).
-Proof.
-  hauto l:on use:InterpExt_Fun_nopf rew:db:InterpUniv.
-Qed.
-
 Lemma InterpUnivN_Fun_inv_nopf n A B P  (h : InterpUnivN n (tPi A B) P) :
   exists (PA : tm -> Prop),
     InterpUnivN n A PA /\
@@ -295,34 +369,7 @@ Proof.
   qauto use:InterpExt_Fun_inv_nopf l:on rew:db:InterpUniv.
 Qed.
 
-Lemma InterpExt_deterministic' n m I A PA PB :
-  InterpExt n I A PA ->
-  InterpExt m I A PB ->
-  PA = PB.
-Proof.
-  move => h0 h1.
-  case : (Coq.Arith.Compare_dec.lt_eq_lt_dec m n); first case.
-  - hauto l:on use:InterpExt_cumulative, InterpExt_deterministic.
-  - move => *; subst.
-    sfirstorder use:InterpExt_deterministic.
-  - move => ?.
-    symmetry.
-    hauto l:on use:InterpExt_cumulative, InterpExt_deterministic.
-Qed.
-
-Lemma InterpUnivN_cumulative n A PA :
-  InterpUnivN n A PA -> forall m, n < m ->
-  InterpUnivN m A PA.
-Proof.
-  hauto l:on rew:db:InterpUniv use:InterpExt_cumulative.
-Qed.
-
-Lemma InterpUnivN_deterministic' n m  A PA PB :
-  InterpUnivN n A PA ->
-  InterpUnivN m A PB ->
-  PA = PB.
-Proof. hauto lq:on rew:off use:InterpExt_deterministic' rew:db:InterpUniv. Qed.
-
+(* ----  Backward closure for the interpreted sets ----- *)
 Lemma InterpUnivN_back_clos n A PA :
     InterpUnivN n A PA ->
     forall a b, Par a b ->
